\documentclass[21pt,a4paper,twoside]{article}
\usepackage{amsmath}
\usepackage{mathtools}

\begin{document}\Large
\begin{equation}
	 S = \min \sum_{i = 1}^{n} (ax_i^2 + bx_i + c - y_i)^2
\end{equation}
	\newline
	\begin{equation}
		\frac{\partial S}{\partial a} = \sum_{i=1}^{n} \not{2} (ax_i^2 + bx_i + c - y_i) x_i^2 = 0
	\end{equation}
	% \begin{equation}
	% 	\frac{\partial S}{\partial b} = \sum_{i=1}^{n} \not{2} (ax_i^2 + bx_i + c - y_i) x_i = 0
	% \end{equation}
	% \begin{equation}
	% 	\frac{\partial S}{\partial c} = \sum_{i=1}^{n} \not{2} (ax_i^2 + bx_i + c - y_i) = 0
	% \end{equation}
	\newline
	\begin{equation}
		\frac{\partial S}{\partial a} = \sum_{i=1}^{n} (ax_i^2 + bx_i + c) x_i^2 - \sum_{i=1}^{n} x_i^2 y_i = 0
	\end{equation}
	% \begin{equation}
	% 	\frac{\partial S}{\partial b} = \sum_{i=1}^{n} (ax_i^2 + bx_i + c) x_i - \sum_{i=1}^{n} x_i y_i = 0
	% \end{equation}
	% \begin{equation}
	% 	\frac{\partial S}{\partial c} = \sum_{i=1}^{n} (ax_i^2 + bx_i + c) - \sum_{i=1}^{n} y_i = 0
	% \end{equation}
	\newline
	\begin{equation}
		\frac{\partial S}{\partial a} = a\sum_{i=1}^{n} ax_i^4 + b\sum_{i=1}^{n} x_i^3 + c\sum_{i=1}^{n} x_i^2 = \sum_{i=1}^{n} x_i^2 y_i
	\end{equation}
	% \begin{equation}
	% 	\frac{\partial S}{\partial b} = a\sum_{i=1}^{n} ax_i^3 + b\sum_{i=1}^{n} x_i^2 + c\sum_{i=1}^{n} x_i = \sum_{i=1}^{n} x_i y_i
	% \end{equation}
	% \begin{equation}
	% 	\frac{\partial S}{\partial c} = a\sum_{i=1}^{n} ax_i^2 + b\sum_{i=1}^{n} x_i + cn = \sum_{i=1}^{n} y_i
	% \end{equation}
	\newline
	\begin{equation}
	\text{Å·}_{T+1} = y_N + \frac{y_N-y_S}{t_N-t_S} (t_{N+1}-t_N)
	\end{equation}
	\[    % <-- start math environment
	\begin{bmatrix*}[l]
		\sum_{i=1}^{n} x_i^4 & \sum_{i=1}^{n} x_i^3 & \sum_{i=1}^{n} x_i^2 \\
		\sum_{i=1}^{n} x_i^3 & \sum_{i=1}^{n} x_i^2 & \sum_{i=1}^{n} x_i \\
		\sum_{i=1}^{n} x_i^2 & \sum_{i=1}^{n} x_i & n
	\end{bmatrix*}
	\begin{bmatrix*}[l]
		a \\
		b \\
		c
	\end{bmatrix*}
	=
	\begin{bmatrix*}[l]
		\sum_{i=1}^{n} x_i^2 y_i \\
		\sum_{i=1}^{n} x_i y_i \\
		\sum_{i=1}^{n} y_i
	\end{bmatrix*}
	% (11)
	\] 
\end{document}